% !TEX root = ../notes.tex

\section{More Noether Theory}

\subsection{Noethers Theorem for EL equations}

Consider $L(\vec q,\, \dot{\vec q})$ for $\vec q \in \R^3$ and $\dot{\vec q} \in T_{\vec q}\R^3$. Suppose that $L$ is left invariant with respect to the tangent lift on $\SO(3)$, ie. $R\in\SO(3)$ with $L(R\vec q\, R\dot{\vec q}) = L(\vec q,\,\dot{\vec q})$. Then we can prove that,
$$ \mathcal{E} := \dit \pd{L}{\dot{\vec q}} - \pd{L}{\vec q} = 0 $$

Now we have theorem,
\begin{nthm}
  Corresponding to each one-parameter subgroup of $\SO(3)$ $R(s)$ where $R(0) = e$ and $R'(0) = \hat\xi \in \mathfrak{SO}(3)$. There is a conserved quantity,
  $$ A_\xi := \ip{\vec q \ti \pd{L}{\dot q}}{\xi} $$
  with $\di{A_\xi}{t} = 0$ along solutions of the Euler Legrange equations $\mathsc{E}(\vec q) = 0$
\end{nthm}
\begin{proof}
  Associated with the one parameter subgroup $R(s)$ is the generator $\xi_{\mathcal{M}}(\vec q) := \di{}{s}_{s=0} R(s)\vec q = \hat\xi \vec q = \xi\ti\vec q$ where $\mathcal{M} = \R^3$. Now we consider,
  \begin{align*}
    \int_{t_1}^{t_2} L(R(s)\vec q,\,R(s)q) = \int_{t_1}^{t_2} L(q,\,\dot q) \,dt \\
  \end{align*}
  and now we differentiate this wrt $s$ and then set $s = 0$ to obtain
  $$ \ip{\pd{L}{\dot q}}{\xi_{\mathcal{M}}(\vec q)} = \dit{\pd{L}{\dot q}}{\xi \ti \vec q} = \ip{\vec q \ti \pd{L}{\dot q}}{\xi} = A_\xi$$
\end{proof}

\subsection{Noether Theory and EP Reduction}
We have,
$$ \int_{t_1}^{t_2} L(R,\,\dot R)\,dt = 0 $$
and $L$ is left-invariant and so, $L(SR,\,S\dot R) = L(R,\,\dot R)$
\begin{nthm}[Noethers Theorem]
  Corresponding to each one parameter subgroup of $\SO(3)$, $S(s)$ with $S(0)= e$ and $S'(0) = \hat\xi \in \mathfrak{SO}(3)$, then there is a conserved quantity
  $$ A_\xi := \ip{\Ad^*_{R^\top}\pd{\hat\ell}{\Oh}}{\hat\xi} $$
  with $\di{A_\xi}{t} = 0$ along solutions of the Euler Lagrange Equation.
  $$ \mathsc{E}(R) := \dit\pd{L}{\dot R} - \pd{L}{R} = \vec 0 $$
\end{nthm}
\begin{proof}
  Consider $S(s)$ and differentiate and let $s = 0$ much like before,
  $$ \int_{t_1}^{t_2} \pd{}{\xi_{\mathcal{M}(R)}}\pd{L}{R} + \ip{\pd{L}{\dot R}}{\xi_{\mathcal{M}(\dot R)}} $$
  where here $\xi_{\mathcal{M}}(R) = \hat\xi R$
\end{proof}
